new_example/calendar.go
@@ -3,19 +3,23 @@ package main
 import "github.com/tchajed/marshal"
 
 type Calendar struct {
+	hash   []byte
 	events []Event
 }
 
 func MarshalCalendar(enc []byte, c Calendar) []byte {
+	enc = marshal.WriteLenPrefixedBytes(enc, c.hash)
 	enc = marshal.WriteInt(enc, uint64(len(c.events)))
 	return marshal.WriteSlice[Event](enc, c.events, MarshalEvent)
 }
 
 func UnmarshalCalendar(s []byte) (Calendar, []byte) {
+	hash, s := marshal.ReadLenPrefixedBytes(s)
 	eventsLen, s := marshal.ReadInt(s)
 	events, s := marshal.ReadSlice[Event](s, eventsLen, UnmarshalEvent)
 
 	return Calendar{
+		hash:   hash,
 		events: events,
 	}, s
 }
