new_example/pg/github_com/mjschwenne/grackle/new_example.v
@@ -15,6 +15,7 @@ Module Calendar.
 Section def.
 Context `{ffi_syntax}.
 Record t := mk {
+  hash' : slice.t;
   events' : slice.t;
 }.
 End def.
@@ -24,39 +25,45 @@ Section instances.
 Context `{ffi_syntax}.
 
 Global Instance settable_Calendar : Settable Calendar.t :=
-  settable! Calendar.mk < Calendar.events' >.
+  settable! Calendar.mk < Calendar.hash'; Calendar.events' >.
 Global Instance into_val_Calendar : IntoVal Calendar.t :=
   {| to_val_def v :=
     struct.val_aux main.Calendar [
+    "hash" ::= #(Calendar.hash' v);
     "events" ::= #(Calendar.events' v)
     ]%struct
   |}.
 
 Global Program Instance into_val_typed_Calendar : IntoValTyped Calendar.t main.Calendar :=
 {|
-  default_val := Calendar.mk (default_val _);
+  default_val := Calendar.mk (default_val _) (default_val _);
 |}.
 Next Obligation. solve_to_val_type. Qed.
 Next Obligation. solve_zero_val. Qed.
 Next Obligation. solve_to_val_inj. Qed.
 Final Obligation. solve_decision. Qed.
 
+Global Instance into_val_struct_field_Calendar_hash : IntoValStructField "hash" main.Calendar Calendar.hash'.
+Proof. solve_into_val_struct_field. Qed.
+
 Global Instance into_val_struct_field_Calendar_events : IntoValStructField "events" main.Calendar Calendar.events'.
 Proof. solve_into_val_struct_field. Qed.
 
 
 Context `{!ffi_model, !ffi_semantics _ _, !ffi_interp _, !heapGS Σ}.
-Global Instance wp_struct_make_Calendar events':
+Global Instance wp_struct_make_Calendar hash' events':
   PureWp True
     (struct.make #main.Calendar (alist_val [
+      "hash" ::= #hash';
       "events" ::= #events'
     ]))%struct
-    #(Calendar.mk events').
+    #(Calendar.mk hash' events').
 Proof. solve_struct_make_pure_wp. Qed.
 
 
 Global Instance Calendar_struct_fields_split dq l (v : Calendar.t) :
   StructFieldsSplit dq l v (
+    "Hhash" ∷ l ↦s[main.Calendar :: "hash"]{dq} v.(Calendar.hash') ∗
     "Hevents" ∷ l ↦s[main.Calendar :: "events"]{dq} v.(Calendar.events')
   ).
 Proof.
@@ -65,6 +72,7 @@ Proof.
   unfold_typed_pointsto; split_pointsto_app.
 
   rewrite -!/(typed_pointsto_def _ _ _) -!typed_pointsto_unseal.
+  simpl_one_flatten_struct (# (Calendar.hash' v)) main.Calendar "hash"%go.
 
   solve_field_ref_f.
 Qed.
